Experiments/ProofChecking/SRCheckerExe.lean
@@ -17,7 +17,7 @@ import LeanSAT.Data.Cnf
 import LeanSAT.Data.ICnf
 import LeanSAT.Data.Literal
 
-open LeanSAT LeanSAT.Model
+open LeanSAT LeanSAT.Model RangeArray
 
 def printUsage : IO Unit := do
   IO.println "Usage: ./SRChecker <cnf> <lsr> [c]"
@@ -28,6 +28,60 @@ def printUsage : IO Unit := do
   IO.println ""
   IO.println "If no command-line arguments are given, prints this help message."
   IO.println "Reads the CNF and LSR files and checks the LSR proof."
+
+def checkProof (lines : List String) (F : RangeArray ILit) (τ : PPA) (σ : PS) : Except Bool SR.SRState := do
+  lines.foldlM (init := SR.SRState.mk F τ σ) (fun (⟨F, τ, σ⟩ : SR.SRState) line =>
+    match SRParser.parseLSRLine F line with
+    | .error _ => .error false
+    | .ok (_, F, pl) =>
+      match pl with
+      | .inl addLine =>
+        SR.checkLine ⟨F, τ, σ⟩ addLine
+      | .inr delLine =>
+        match SR.consumeDeletionLine F delLine with
+        | .ok F => .ok ⟨F, τ, σ⟩
+        | .error _ => .error false)
+
+def checkProof_error_true {lines : List String}
+    {F : RangeArray ILit} {Ls : List (Option (List ILit))} (h_models : models F Ls [])
+    {τ : PPA} {σ : PS} :
+    checkProof lines F τ σ = .error true → cnfListToPropFun Ls = ⊥ := by
+  induction lines generalizing F Ls τ σ with
+  | nil => simp [checkProof, pure, Except.pure]
+  | cons line lines ih =>
+    simp [checkProof]
+    split
+    · simp [bind, Except.bind]
+    · rename_i lineId F' parsedLine parseRes
+      split
+      · rename_i addLine
+        rcases SRParser.parseLSRLine_ok_inl parseRes h_models with ⟨C, hC⟩
+        simp [bind, Except.bind]
+        split
+        · rename_i b h_checkLine
+          cases b <;> simp
+          have := SR.checkLine_error_true hC h_checkLine
+          simp at this
+          exact this
+        · rename_i S h_checkLine
+          rcases SR.checkLine_ok hC h_checkLine with ⟨⟨τ', σ', hS⟩, h₂⟩
+          subst hS
+          have h_models_commit := models_commit hC
+          intro h
+          have := ih h_models_commit h
+          simp [LeanColls.Seq.snoc] at this
+          simp at h₂
+          exact (PropFun.eq_bot_iff_eq_bot_of_eqsat h₂).mpr this
+      · rename_i delLine
+        have := SRParser.parseLSRLine_ok_inr parseRes
+        subst this
+        split
+        · rename_i F₂ h_consumeDeletionLine
+          rcases SR.consumeDeletionLine_ok h_models h_consumeDeletionLine with ⟨Ls₂, h_models₂, h_toPropFun⟩
+          intro h
+          rw [ih h_models₂ h, le_bot_iff] at h_toPropFun
+          exact h_toPropFun
+        · simp [bind, Except.bind]
 
 def interpretResult : Except Bool SRState → IO Unit
   | .ok _ => do
@@ -49,20 +103,8 @@ partial def main : List String → IO Unit
 
     let lsrContents ← IO.FS.withFile lsrFile .read (·.readToEnd)
     let lines := lsrContents.splitOn "\n"
-    interpretResult <| lines.foldlM (init := SR.SRState.mk F (PPA.new (nvars * 2)) (PS.new (nvars * 2))) (fun ⟨F, τ, σ⟩ line =>
-      match SRParser.parseLSRLine F line with
-      | .error _ =>
-        -- dbg_trace s!"Error: {str}"
-        .error false
-      | .ok (_, F, pl) =>
-        -- dbg_trace s!"Parsed line with id {id}"
-        match pl with
-        | .inl addLine =>
-          SR.checkLine ⟨F, τ, σ⟩ addLine
-        | .inr delLine =>
-          match SR.consumeDeletionLine F delLine with
-          | .ok F => .ok ⟨F, τ, σ⟩
-          | .error _ => .error false)
+    interpretResult <| checkProof lines F (PPA.new (nvars * 2)) (PS.new (nvars * 2))
+
   | [cnfFile, lsrFile, "c"] => do
     let cnfContents ← IO.FS.withFile cnfFile .read (·.readToEnd)
     let (F, nvars) ← IO.ofExcept <| SRParser.parseFormula cnfContents (RangeArray.empty : RangeArray ILit)
@@ -73,11 +115,8 @@ partial def main : List String → IO Unit
     | ⟨F, τ, σ⟩ => do
       if index < b_size then
         match SRParser.parseLSRLineBinary F bytes index with
-        | .error _ =>
-          -- dbg_trace s!"Error: {str}"
-          .error false
+        | .error _ => .error false
         | .ok (index, _, F, pl) =>
-          -- dbg_trace s!"Parsed line with id {id}"
           --let F := F.commitUntil (id - 1)
           match pl with
           | .inl addLine =>
