LeanSAT/Data/HashAssn.lean
@@ -9,24 +9,24 @@ import LeanSAT.Data.Cnf
 
 namespace LeanSAT
 
-/-- Partial assignment implementation backed by `Std.HashMap`.
+/-- Partial assignment implementation backed by `Batteries.HashMap`.
 
 Good for sparse partial assignments.
 -/
 def HashAssn (L : Type u) [LitVar L ν] [BEq ν] [Hashable ν] :=
-  Std.HashMap ν Bool
+  Batteries.HashMap ν Bool
 
 namespace HashAssn
 
 variable {L : Type u} {ν : Type v} [LitVar L ν] [BEq ν] [Hashable ν]
 
-def empty : HashAssn L := Std.HashMap.empty
+def empty : HashAssn L := Batteries.HashMap.empty
 
 variable (self : HashAssn L)
 
-def set (l : L) : HashAssn L := Std.HashMap.insert self (LitVar.toVar l) (LitVar.polarity l)
+def set (l : L) : HashAssn L := Batteries.HashMap.insert self (LitVar.toVar l) (LitVar.polarity l)
 
-def toLitArray : Array L := Std.HashMap.toArray self |>.map (fun (a,b) => LitVar.mkLit L a b)
+def toLitArray : Array L := Batteries.HashMap.toArray self |>.map (fun (a,b) => LitVar.mkLit L a b)
 
 instance [ToString L] : ToString (HashAssn L) where
   toString a := a.fold (fun s v b => s ++ toString (LitVar.mkLit L v b)) ""
